# 单链表的插入验证

$$
\{list\;\overline{\gamma}\;(head)\}\\
seqInsert\;(head;val)\;\{\}\\
\{\exists \alpha, \beta,list\;\overline{\alpha\cdot val\cdot\beta}\;(head)\wedge\alpha\cdot\beta=\gamma \}\\
$$


```cpp
void insert(List* list, int val) {
    if(list->head == NULL) {  
        list->head = new ListNode(val);
    } else if(list->head->data >= val){
        list->head = new ListNode(val, list->head);
    } else {
        ListNode* former = list->head;
        ListNode* cur = former->next;
        while(cur != NULL && val > cur->data){
            former = cur;
            cur = cur->next;
        }
        former->next = new ListNode(val, cur);
    }
}
```

```python
if head == nil:
    head = cons(val, nil)
else if [head] >= val:
    tmp = cons(val, head)
    head = tmp
else:
    former = head
    cur = [former+1]
    while cur != nil && val > [cur]:
        former = cur
        tmp = [cur+1]
        cur = tmp
    next = cons(val, cur)
    [former+1] = next
```

$$
\{list\;\overline{\gamma}\;(head)\}\\
if\;head == nil:\\
\{list\;\overline{\gamma}\;(head)\;\wedge\;head=nil\}\\
\{emp\;\wedge\;\gamma = \epsilon\}\\
head = cons(val,nil)\\
\{head\mapsto val, nil\;\wedge\;\gamma = \epsilon\}\\
\{list\;val\;head\;\wedge\;\gamma = \epsilon\}\\
\{list\;\overline{\epsilon\cdot val\cdot\epsilon}\;head\;\wedge\;\gamma = \epsilon\}\\
\{\exists \alpha, \beta,list\;\overline{\alpha\cdot val\cdot\beta}\;(head)\wedge\alpha\cdot\beta=\gamma \}\\
$$

$$
else\;if\;[head] \ge val:\\
\{list\;\overline{\gamma}\;(head)\;\wedge\;head\ne nil\;\wedge\;[head] \ge val\}\\  % \alpha \ne \epsilon
\{\exists a,\beta'.\; list\;a\cdot\beta' \;head\;\wedge\;a\cdot\beta' = \overline{\gamma}\;\wedge\;[head] \ge val \}\\
\{\exists a,\beta'.\; list\;a\cdot\beta' \;head\;\wedge\;a\cdot\beta' = \overline{\gamma}\;\wedge\;a \ge val \}\\
\{list\;\overline{\gamma} \;head\;\wedge\;\gamma_{1} \ge val  \}\\  
tmp = cons(val, head)\\
\{tmp\mapsto val, head\;*\;list\;\overline{\gamma} \;head\;\wedge\;\gamma_{1} \ge val\}\\
\{list\;val\cdot\overline{\gamma} \;tmp\;\wedge\;\gamma_{1} \ge val\}\\
\{list\;\overline{val\cdot{\gamma}} \;tmp\}\\
head = tmp\\
\{list\;\overline{val\cdot{\gamma}} \;head\}\\
\{list\;\overline{\epsilon\cdot val\cdot{\gamma}} \;head\;\wedge\;\epsilon\cdot\gamma = \gamma\}\\
\{\exists \alpha, \beta,list\;\overline{\alpha\cdot val\cdot\beta}\;(head)\wedge\alpha\cdot\beta=\gamma \}\\
$$

$$
else:\\
\{list\;\overline{\gamma}\;(head)\;\wedge\;head\ne nil\;\wedge\; [head] \lt val\}\\
\{list\;\overline{\gamma}\;(head)\;\wedge\;head\ne nil\;\wedge\; [head] \lt val\;\wedge\;head = head\}\\
    former = head\\
\{list\;\overline{\gamma}\;(head)\;\wedge\;head\ne nil\;\wedge\; [head] \lt val\;\wedge\;former = head\}\\
\{\exists \gamma'.\;list\;\overline{a\cdot\gamma'}\;(head)\;\wedge\;a\cdot\gamma'=\gamma\;\wedge\;head\ne nil\;\wedge\; [head] \lt val\;\wedge\;former = head\}\\
% 可以拆开
\{\exists \gamma'.\;list\;a\cdot\gamma'\;(head)\;\wedge\;a\cdot\gamma'=\overline{\gamma}\;\wedge\; a \lt val\;\wedge\;former = head\}\\
\{\exists \gamma',a,next.\; lseg\;\epsilon\;(head, former)\;*\; former\mapsto a,next\;*\;lseg\;\gamma'\;(next, nil)\;\wedge\;a\cdot\gamma'=\overline{\gamma}\;\wedge\; a \lt val\;\wedge\;former = head\}\\

    cur = [former + 1]\\

\{\exists \gamma',a.\; lseg\;\epsilon\;(head, former)\;*\; former\mapsto a,cur\;*\;lseg\;\gamma'\;(cur, nil)\;\wedge\;a\cdot\gamma'=\overline{\gamma}\;\wedge\; a \lt val\;\wedge\;former = head\}\\

\{\exists \alpha',a,\beta.\; lseg\;\alpha'\;(head, former)\;*\; former\mapsto a,cur\;*\;lseg\;\beta\;(cur, nil)\;\wedge\;\alpha'\cdot a\cdot\beta = \overline{\gamma}\;\wedge\; a \lt val\}\\

    while\;cur \ne nil\;\wedge\;val > [cur]:\\

\{\exists \alpha',a,\beta.\; lseg\;\alpha'\;(head, former)\;*\; former\mapsto a,cur\;*\;lseg\;\beta\;(cur, nil)\;\wedge\;\alpha'\cdot a\cdot\beta = \overline{\gamma}\;\wedge\; a \lt val\;\wedge\;cur\ne nil\;\wedge\;val > [cur]\}\\

\{\exists \alpha',a,b,\beta'.\; lseg\;\alpha'\;(head, former)\;*\; former\mapsto a,cur\;*\;lseg\;b\cdot\beta'\;(cur, nil)\;\wedge\;\alpha'\cdot a\cdot b\cdot\beta' = \overline{\gamma}\;\wedge\; a \lt val\;\wedge\;cur\ne nil\;\wedge\;val > [cur]\}\\

\{\exists \alpha',a,b,\beta'.\; lseg\;\alpha'\cdot a\;(head, cur)\;*\;lseg\;b\cdot\beta'\;(cur, nil)\;\wedge\;\alpha'\cdot a\cdot b\cdot\beta' = \overline{\gamma}\;\wedge\; b < val\;\wedge\;cur\ne nil\}\\

\{\exists \alpha',a,b,\beta',next.\; lseg\;\alpha'\cdot a\;(head, cur)\;*\;cur\mapsto b,next\;*\;lseg\;\beta'\;(next, nil)\;\wedge\;\alpha'\cdot a\cdot b\cdot\beta' = \overline{\gamma}\;\wedge\; b < val\}\\

        former = cur\\

\{\exists \alpha',a,b,\beta',next.\; lseg\;\alpha'\cdot a\;(head, former)\;*\;former\mapsto b,next\;*\;lseg\;\beta'\;(next, nil)\;\wedge\;\alpha'\cdot a\cdot b\cdot\beta' = \overline{\gamma}\;\wedge\; b < val\;\wedge\;former = cur\}\\

\{\exists \alpha',b,\beta',next.\; lseg\;\alpha'\;(head, former)\;*\;former\mapsto b,next\;*\;lseg\;\beta'\;(next, nil)\;\wedge\;\alpha'\cdot b\cdot\beta' = \overline{\gamma}\;\wedge\; b < val\;\wedge\;former = cur\}\\

        tmp = [cur+1]\\

\{\exists \alpha',b,\beta'.\; lseg\;\alpha'\;(head, former)\;*\; former\mapsto b,tmp\;*\;lseg\;\beta'\;(tmp, nil)\;\wedge\;\alpha'\cdot b\cdot\beta' = \overline{\gamma}\;\wedge\; b \lt val\}\\

        cur = tmp\\

\{\exists \alpha',b,\beta'.\; lseg\;\alpha'\;(head, former)\;*\; former\mapsto b,cur\;*\;lseg\;\beta'\;(cur, nil)\;\wedge\;\alpha'\cdot b\cdot\beta' = \overline{\gamma}\;\wedge\; b \lt val\}\\
    
\{\exists \alpha',a,\beta.\; lseg\;\alpha'\;(head, former)\;*\; former\mapsto a,cur\;*\;lseg\;\beta\;(cur, nil)\;\wedge\;\alpha'\cdot a\cdot\beta = \overline{\gamma}\;\wedge\; a \lt val\}\\

    end\;while\\


\{\exists \alpha',a,\beta.\; lseg\;\alpha'\;(head, former)\;*\; former\mapsto a,cur\;*\;lseg\;\beta\;(cur, nil)\;\wedge\;\alpha'\cdot a\cdot\beta = \overline{\gamma}\;\wedge\; a \lt val\;\wedge\;(cur = nil\;\vee\;val \le [cur])\}\\

    next = cons(val, cur)\\

\{\exists \alpha',a,\beta.\; lseg\;\alpha'\;(head, former)\;*\; former\mapsto a,cur\;*\;next \mapsto val, cur\;*\;lseg\;\beta\;(cur, nil)\;\wedge\;\alpha'\cdot a\cdot\beta = \overline{\gamma}\;\wedge\; a \lt val\;\wedge\;(cur = nil\;\vee\;val \le [cur])\}\\

    [former+1] = next\\

\{\exists \alpha',a,\beta.\; lseg\;\alpha'\;(head, former)\;*\; former\mapsto a,next\;*\;next \mapsto val, cur\;*\;lseg\;\beta\;(cur, nil)\;\wedge\;\alpha'\cdot a\cdot\beta = \overline{\gamma}\;\wedge\; a \lt val\;\wedge\;(cur = nil\;\vee\;val \le [cur])\}\\

\{\exists \alpha',a,\beta.\; lseg\;\alpha'\cdot a\cdot val\;(head, cur)\;*\;lseg\;\beta\;(cur, nil)\;\wedge\;\alpha'\cdot a\cdot\beta = \overline{\gamma}\;\wedge\; a \lt val\;\wedge\;(cur = nil\;\vee\;val \le [cur])\}\\
$$

$$
\{\exists \alpha,\beta.\; lseg\;\alpha\cdot val\;(head, cur)\;*\;lseg\;\beta\;(cur, nil)\;\wedge\;\alpha\cdot\beta = \overline{\gamma}\;\wedge\; \alpha_{-1} \lt val\;\wedge\;(cur = nil\;\vee\;val \le [cur])\}\\

\{\exists \alpha,\beta.\; lseg\;\alpha\cdot val\;(head, cur)\;*\;lseg\;\beta\;(cur, nil)\;\wedge\;\alpha\cdot\beta = \overline{\gamma}\;\wedge\; \alpha_{-1} \lt val\;\wedge\;(\beta = \epsilon\;\vee\;val \le \beta_1)\}\\

\{\exists \alpha,\beta.\; lseg\;\alpha\cdot val\;(head, cur)\;*\;lseg\;\beta\;(cur, nil)\;\wedge\;\alpha\cdot\beta = \overline{\gamma}\;\wedge\; (\alpha = \epsilon \;\vee\;\alpha_{-1} \lt val)\;\wedge\;(\beta = \epsilon\;\vee\;val \le \beta_1)\}\\

\{\exists \alpha,\beta.\; lseg\;\overline{\alpha}\cdot val\;(head, cur)\;*\;lseg\;\overline{\beta}\;(cur, nil)\;\wedge\;\alpha\cdot\beta = \gamma\;\wedge\; (\alpha = \epsilon \;\vee\;\alpha_{-1} \lt val)\;\wedge\;(\beta = \epsilon\;\vee\;val \le \beta_1)\}\\

\{\exists \alpha,\beta.\; lseg\;\overline{\alpha}\cdot val\cdot\overline{\beta}\;(head, nil)\;\wedge\;\alpha\cdot\beta = \gamma\;\wedge\; (\alpha = \epsilon \;\vee\;\alpha_{-1} \lt val)\;\wedge\;(\beta = \epsilon\;\vee\;val \le \beta_1)\}\\

\{\exists \alpha, \beta,list\;\overline{\alpha\cdot val\cdot\beta}\;(head)\wedge\alpha\cdot\beta=\gamma \}\\
$$
